libcrux-ml-kem/proofs/fstar/extraction/Libcrux_ml_kem.Simd.Portable.fsti
@@ -5,914 +5,189 @@ open FStar.Mul
 
 type t_PortableVector = { f_elements:t_Array i32 (sz 8) }
 
+val v_ZERO: Prims.unit -> Prims.Pure t_PortableVector Prims.l_True (fun _ -> Prims.l_True)
+
+val add (lhs rhs: t_PortableVector)
+    : Prims.Pure t_PortableVector Prims.l_True (fun _ -> Prims.l_True)
+
+val add_constant (v: t_PortableVector) (c: i32)
+    : Prims.Pure t_PortableVector Prims.l_True (fun _ -> Prims.l_True)
+
+val barrett_reduce (v: t_PortableVector)
+    : Prims.Pure t_PortableVector Prims.l_True (fun _ -> Prims.l_True)
+
+val bitwise_and_with_constant (v: t_PortableVector) (c: i32)
+    : Prims.Pure t_PortableVector Prims.l_True (fun _ -> Prims.l_True)
+
+val compress (coefficient_bits: u8) (v: t_PortableVector)
+    : Prims.Pure t_PortableVector Prims.l_True (fun _ -> Prims.l_True)
+
+val compress_1_ (v: t_PortableVector)
+    : Prims.Pure t_PortableVector Prims.l_True (fun _ -> Prims.l_True)
+
+val from_i32_array (array: t_Array i32 (sz 8))
+    : Prims.Pure t_PortableVector Prims.l_True (fun _ -> Prims.l_True)
+
+val inv_ntt_layer_1_step (v: t_PortableVector) (zeta1 zeta2: i32)
+    : Prims.Pure t_PortableVector Prims.l_True (fun _ -> Prims.l_True)
+
+val inv_ntt_layer_2_step (v: t_PortableVector) (zeta: i32)
+    : Prims.Pure t_PortableVector Prims.l_True (fun _ -> Prims.l_True)
+
+val modulo_a_constant (v: t_PortableVector) (modulus: i32)
+    : Prims.Pure t_PortableVector Prims.l_True (fun _ -> Prims.l_True)
+
+val montgomery_reduce (v: t_PortableVector)
+    : Prims.Pure t_PortableVector Prims.l_True (fun _ -> Prims.l_True)
+
+val multiply_by_constant (v: t_PortableVector) (c: i32)
+    : Prims.Pure t_PortableVector Prims.l_True (fun _ -> Prims.l_True)
+
+val ntt_layer_1_step (v: t_PortableVector) (zeta1 zeta2: i32)
+    : Prims.Pure t_PortableVector Prims.l_True (fun _ -> Prims.l_True)
+
+val ntt_layer_2_step (v: t_PortableVector) (zeta: i32)
+    : Prims.Pure t_PortableVector Prims.l_True (fun _ -> Prims.l_True)
+
+val serialize_1_ (v: t_PortableVector) : Prims.Pure u8 Prims.l_True (fun _ -> Prims.l_True)
+
+val serialize_10_ (v: t_PortableVector)
+    : Prims.Pure (t_Array u8 (sz 10)) Prims.l_True (fun _ -> Prims.l_True)
+
+val serialize_11_ (v: t_PortableVector)
+    : Prims.Pure (t_Array u8 (sz 11)) Prims.l_True (fun _ -> Prims.l_True)
+
+val serialize_12_ (v: t_PortableVector)
+    : Prims.Pure (t_Array u8 (sz 12)) Prims.l_True (fun _ -> Prims.l_True)
+
+val serialize_4_ (v: t_PortableVector)
+    : Prims.Pure (t_Array u8 (sz 4)) Prims.l_True (fun _ -> Prims.l_True)
+
+val serialize_5_ (v: t_PortableVector)
+    : Prims.Pure (t_Array u8 (sz 5)) Prims.l_True (fun _ -> Prims.l_True)
+
+val shift_left (lhs: t_PortableVector) (shift_amount: u8)
+    : Prims.Pure t_PortableVector Prims.l_True (fun _ -> Prims.l_True)
+
+val shift_right (v: t_PortableVector) (shift_amount: u8)
+    : Prims.Pure t_PortableVector Prims.l_True (fun _ -> Prims.l_True)
+
+val sub (lhs rhs: t_PortableVector)
+    : Prims.Pure t_PortableVector Prims.l_True (fun _ -> Prims.l_True)
+
+val to_i32_array (v: t_PortableVector)
+    : Prims.Pure (t_Array i32 (sz 8)) Prims.l_True (fun _ -> Prims.l_True)
+
+val deserialize_1_ (v: u8) : Prims.Pure t_PortableVector Prims.l_True (fun _ -> Prims.l_True)
+
+val deserialize_10_ (bytes: t_Slice u8)
+    : Prims.Pure t_PortableVector Prims.l_True (fun _ -> Prims.l_True)
+
+val deserialize_11_ (bytes: t_Slice u8)
+    : Prims.Pure t_PortableVector Prims.l_True (fun _ -> Prims.l_True)
+
+val deserialize_12_ (bytes: t_Slice u8)
+    : Prims.Pure t_PortableVector Prims.l_True (fun _ -> Prims.l_True)
+
+val deserialize_4_ (bytes: t_Slice u8)
+    : Prims.Pure t_PortableVector Prims.l_True (fun _ -> Prims.l_True)
+
+val deserialize_5_ (bytes: t_Slice u8)
+    : Prims.Pure t_PortableVector Prims.l_True (fun _ -> Prims.l_True)
+
+val ntt_multiply (lhs rhs: t_PortableVector) (zeta0 zeta1: i32)
+    : Prims.Pure t_PortableVector Prims.l_True (fun _ -> Prims.l_True)
+
 [@@ FStar.Tactics.Typeclasses.tcinstance]
-let impl: Libcrux_ml_kem.Simd.Simd_trait.t_ArrayOperations t_PortableVector =
+let impl: Libcrux_ml_kem.Simd.Simd_trait.t_Operations t_PortableVector =
   {
     f_ZERO_pre = (fun (_: Prims.unit) -> true);
     f_ZERO_post = (fun (_: Prims.unit) (out: t_PortableVector) -> true);
-    f_ZERO
-    =
-    (fun (_: Prims.unit) ->
-        { f_elements = Rust_primitives.Hax.repeat 0l (sz 8) } <: t_PortableVector);
+    f_ZERO = (fun (_: Prims.unit) -> v_ZERO ());
     f_to_i32_array_pre = (fun (v: t_PortableVector) -> true);
     f_to_i32_array_post = (fun (v: t_PortableVector) (out: t_Array i32 (sz 8)) -> true);
-    f_to_i32_array = (fun (v: t_PortableVector) -> v.f_elements);
+    f_to_i32_array = (fun (v: t_PortableVector) -> to_i32_array v);
     f_from_i32_array_pre = (fun (array: t_Array i32 (sz 8)) -> true);
     f_from_i32_array_post = (fun (array: t_Array i32 (sz 8)) (out: t_PortableVector) -> true);
-    f_from_i32_array = fun (array: t_Array i32 (sz 8)) -> { f_elements = array } <: t_PortableVector
-  }
-
-[@@ FStar.Tactics.Typeclasses.tcinstance]
-let impl_1: Libcrux_ml_kem.Simd.Simd_trait.t_ArithmeticOperations t_PortableVector =
-  {
+    f_from_i32_array = (fun (array: t_Array i32 (sz 8)) -> from_i32_array array);
     f_add_constant_pre = (fun (v: t_PortableVector) (c: i32) -> true);
     f_add_constant_post = (fun (v: t_PortableVector) (c: i32) (out: t_PortableVector) -> true);
-    f_add_constant
-    =
-    (fun (v: t_PortableVector) (c: i32) ->
-        let v:t_PortableVector =
-          Core.Iter.Traits.Iterator.f_fold (Core.Iter.Traits.Collect.f_into_iter ({
-                    Core.Ops.Range.f_start = sz 0;
-                    Core.Ops.Range.f_end = Libcrux_ml_kem.Simd.Simd_trait.v_FIELD_ELEMENTS_IN_VECTOR
-                  }
-                  <:
-                  Core.Ops.Range.t_Range usize)
-              <:
-              Core.Ops.Range.t_Range usize)
-            v
-            (fun v i ->
-                let v:t_PortableVector = v in
-                let i:usize = i in
-                {
-                  v with
-                  f_elements
-                  =
-                  Rust_primitives.Hax.Monomorphized_update_at.update_at_usize v.f_elements
-                    i
-                    ((v.f_elements.[ i ] <: i32) +! c <: i32)
-                  <:
-                  t_Array i32 (sz 8)
-                }
-                <:
-                t_PortableVector)
-        in
-        v);
+    f_add_constant = (fun (v: t_PortableVector) (c: i32) -> add_constant v c);
     f_add_pre = (fun (lhs: t_PortableVector) (rhs: t_PortableVector) -> true);
     f_add_post
     =
     (fun (lhs: t_PortableVector) (rhs: t_PortableVector) (out: t_PortableVector) -> true);
-    f_add
-    =
-    (fun (lhs: t_PortableVector) (rhs: t_PortableVector) ->
-        let lhs:t_PortableVector =
-          Core.Iter.Traits.Iterator.f_fold (Core.Iter.Traits.Collect.f_into_iter ({
-                    Core.Ops.Range.f_start = sz 0;
-                    Core.Ops.Range.f_end = Libcrux_ml_kem.Simd.Simd_trait.v_FIELD_ELEMENTS_IN_VECTOR
-                  }
-                  <:
-                  Core.Ops.Range.t_Range usize)
-              <:
-              Core.Ops.Range.t_Range usize)
-            lhs
-            (fun lhs i ->
-                let lhs:t_PortableVector = lhs in
-                let i:usize = i in
-                {
-                  lhs with
-                  f_elements
-                  =
-                  Rust_primitives.Hax.Monomorphized_update_at.update_at_usize lhs.f_elements
-                    i
-                    ((lhs.f_elements.[ i ] <: i32) +! (rhs.f_elements.[ i ] <: i32) <: i32)
-                  <:
-                  t_Array i32 (sz 8)
-                }
-                <:
-                t_PortableVector)
-        in
-        lhs);
+    f_add = (fun (lhs: t_PortableVector) (rhs: t_PortableVector) -> add lhs rhs);
     f_sub_pre = (fun (lhs: t_PortableVector) (rhs: t_PortableVector) -> true);
     f_sub_post
     =
     (fun (lhs: t_PortableVector) (rhs: t_PortableVector) (out: t_PortableVector) -> true);
-    f_sub
-    =
-    (fun (lhs: t_PortableVector) (rhs: t_PortableVector) ->
-        let lhs:t_PortableVector =
-          Core.Iter.Traits.Iterator.f_fold (Core.Iter.Traits.Collect.f_into_iter ({
-                    Core.Ops.Range.f_start = sz 0;
-                    Core.Ops.Range.f_end = Libcrux_ml_kem.Simd.Simd_trait.v_FIELD_ELEMENTS_IN_VECTOR
-                  }
-                  <:
-                  Core.Ops.Range.t_Range usize)
-              <:
-              Core.Ops.Range.t_Range usize)
-            lhs
-            (fun lhs i ->
-                let lhs:t_PortableVector = lhs in
-                let i:usize = i in
-                {
-                  lhs with
-                  f_elements
-                  =
-                  Rust_primitives.Hax.Monomorphized_update_at.update_at_usize lhs.f_elements
-                    i
-                    ((lhs.f_elements.[ i ] <: i32) -! (rhs.f_elements.[ i ] <: i32) <: i32)
-                  <:
-                  t_Array i32 (sz 8)
-                }
-                <:
-                t_PortableVector)
-        in
-        lhs);
+    f_sub = (fun (lhs: t_PortableVector) (rhs: t_PortableVector) -> sub lhs rhs);
     f_multiply_by_constant_pre = (fun (v: t_PortableVector) (c: i32) -> true);
     f_multiply_by_constant_post
     =
     (fun (v: t_PortableVector) (c: i32) (out: t_PortableVector) -> true);
-    f_multiply_by_constant
-    =
-    fun (v: t_PortableVector) (c: i32) ->
-      let v:t_PortableVector =
-        Core.Iter.Traits.Iterator.f_fold (Core.Iter.Traits.Collect.f_into_iter ({
-                  Core.Ops.Range.f_start = sz 0;
-                  Core.Ops.Range.f_end = Libcrux_ml_kem.Simd.Simd_trait.v_FIELD_ELEMENTS_IN_VECTOR
-                }
-                <:
-                Core.Ops.Range.t_Range usize)
-            <:
-            Core.Ops.Range.t_Range usize)
-          v
-          (fun v i ->
-              let v:t_PortableVector = v in
-              let i:usize = i in
-              {
-                v with
-                f_elements
-                =
-                Rust_primitives.Hax.Monomorphized_update_at.update_at_usize v.f_elements
-                  i
-                  ((v.f_elements.[ i ] <: i32) *! c <: i32)
-                <:
-                t_Array i32 (sz 8)
-              }
-              <:
-              t_PortableVector)
-      in
-      v
-  }
-
-[@@ FStar.Tactics.Typeclasses.tcinstance]
-let impl_2: Libcrux_ml_kem.Simd.Simd_trait.t_BitwiseOperations t_PortableVector =
-  {
+    f_multiply_by_constant = (fun (v: t_PortableVector) (c: i32) -> multiply_by_constant v c);
     f_bitwise_and_with_constant_pre = (fun (v: t_PortableVector) (c: i32) -> true);
     f_bitwise_and_with_constant_post
     =
     (fun (v: t_PortableVector) (c: i32) (out: t_PortableVector) -> true);
     f_bitwise_and_with_constant
     =
-    (fun (v: t_PortableVector) (c: i32) ->
-        let v:t_PortableVector =
-          Core.Iter.Traits.Iterator.f_fold (Core.Iter.Traits.Collect.f_into_iter ({
-                    Core.Ops.Range.f_start = sz 0;
-                    Core.Ops.Range.f_end = Libcrux_ml_kem.Simd.Simd_trait.v_FIELD_ELEMENTS_IN_VECTOR
-                  }
-                  <:
-                  Core.Ops.Range.t_Range usize)
-              <:
-              Core.Ops.Range.t_Range usize)
-            v
-            (fun v i ->
-                let v:t_PortableVector = v in
-                let i:usize = i in
-                {
-                  v with
-                  f_elements
-                  =
-                  Rust_primitives.Hax.Monomorphized_update_at.update_at_usize v.f_elements
-                    i
-                    ((v.f_elements.[ i ] <: i32) &. c <: i32)
-                  <:
-                  t_Array i32 (sz 8)
-                }
-                <:
-                t_PortableVector)
-        in
-        v);
+    (fun (v: t_PortableVector) (c: i32) -> bitwise_and_with_constant v c);
     f_shift_right_pre = (fun (v: t_PortableVector) (shift_amount: u8) -> true);
     f_shift_right_post
     =
     (fun (v: t_PortableVector) (shift_amount: u8) (out: t_PortableVector) -> true);
-    f_shift_right
-    =
-    (fun (v: t_PortableVector) (shift_amount: u8) ->
-        let v:t_PortableVector =
-          Core.Iter.Traits.Iterator.f_fold (Core.Iter.Traits.Collect.f_into_iter ({
-                    Core.Ops.Range.f_start = sz 0;
-                    Core.Ops.Range.f_end = Libcrux_ml_kem.Simd.Simd_trait.v_FIELD_ELEMENTS_IN_VECTOR
-                  }
-                  <:
-                  Core.Ops.Range.t_Range usize)
-              <:
-              Core.Ops.Range.t_Range usize)
-            v
-            (fun v i ->
-                let v:t_PortableVector = v in
-                let i:usize = i in
-                {
-                  v with
-                  f_elements
-                  =
-                  Rust_primitives.Hax.Monomorphized_update_at.update_at_usize v.f_elements
-                    i
-                    ((v.f_elements.[ i ] <: i32) >>! shift_amount <: i32)
-                  <:
-                  t_Array i32 (sz 8)
-                }
-                <:
-                t_PortableVector)
-        in
-        v);
-    f_shift_left_pre = (fun (lhs: t_PortableVector) (shift_amount: u8) -> true);
+    f_shift_right = (fun (v: t_PortableVector) (shift_amount: u8) -> shift_right v shift_amount);
+    f_shift_left_pre = (fun (v: t_PortableVector) (shift_amount: u8) -> true);
     f_shift_left_post
     =
-    (fun (lhs: t_PortableVector) (shift_amount: u8) (out: t_PortableVector) -> true);
-    f_shift_left
-    =
-    fun (lhs: t_PortableVector) (shift_amount: u8) ->
-      let lhs:t_PortableVector =
-        Core.Iter.Traits.Iterator.f_fold (Core.Iter.Traits.Collect.f_into_iter ({
-                  Core.Ops.Range.f_start = sz 0;
-                  Core.Ops.Range.f_end = Libcrux_ml_kem.Simd.Simd_trait.v_FIELD_ELEMENTS_IN_VECTOR
-                }
-                <:
-                Core.Ops.Range.t_Range usize)
-            <:
-            Core.Ops.Range.t_Range usize)
-          lhs
-          (fun lhs i ->
-              let lhs:t_PortableVector = lhs in
-              let i:usize = i in
-              {
-                lhs with
-                f_elements
-                =
-                Rust_primitives.Hax.Monomorphized_update_at.update_at_usize lhs.f_elements
-                  i
-                  ((lhs.f_elements.[ i ] <: i32) <<! shift_amount <: i32)
-                <:
-                t_Array i32 (sz 8)
-              }
-              <:
-              t_PortableVector)
-      in
-      lhs
-  }
-
-[@@ FStar.Tactics.Typeclasses.tcinstance]
-let impl_3: Libcrux_ml_kem.Simd.Simd_trait.t_ModularOperations t_PortableVector =
-  {
+    (fun (v: t_PortableVector) (shift_amount: u8) (out: t_PortableVector) -> true);
+    f_shift_left = (fun (v: t_PortableVector) (shift_amount: u8) -> shift_left v shift_amount);
     f_modulo_a_constant_pre = (fun (v: t_PortableVector) (modulus: i32) -> true);
     f_modulo_a_constant_post
     =
     (fun (v: t_PortableVector) (modulus: i32) (out: t_PortableVector) -> true);
-    f_modulo_a_constant
-    =
-    (fun (v: t_PortableVector) (modulus: i32) ->
-        let v:t_PortableVector =
-          Core.Iter.Traits.Iterator.f_fold (Core.Iter.Traits.Collect.f_into_iter ({
-                    Core.Ops.Range.f_start = sz 0;
-                    Core.Ops.Range.f_end = Libcrux_ml_kem.Simd.Simd_trait.v_FIELD_ELEMENTS_IN_VECTOR
-                  }
-                  <:
-                  Core.Ops.Range.t_Range usize)
-              <:
-              Core.Ops.Range.t_Range usize)
-            v
-            (fun v i ->
-                let v:t_PortableVector = v in
-                let i:usize = i in
-                {
-                  v with
-                  f_elements
-                  =
-                  Rust_primitives.Hax.Monomorphized_update_at.update_at_usize v.f_elements
-                    i
-                    ((v.f_elements.[ i ] <: i32) %! modulus <: i32)
-                  <:
-                  t_Array i32 (sz 8)
-                }
-                <:
-                t_PortableVector)
-        in
-        v);
+    f_modulo_a_constant = (fun (v: t_PortableVector) (modulus: i32) -> modulo_a_constant v modulus);
     f_barrett_reduce_pre = (fun (v: t_PortableVector) -> true);
     f_barrett_reduce_post = (fun (v: t_PortableVector) (out: t_PortableVector) -> true);
-    f_barrett_reduce
-    =
-    (fun (v: t_PortableVector) ->
-        let v:t_PortableVector =
-          Core.Iter.Traits.Iterator.f_fold (Core.Iter.Traits.Collect.f_into_iter ({
-                    Core.Ops.Range.f_start = sz 0;
-                    Core.Ops.Range.f_end = Libcrux_ml_kem.Simd.Simd_trait.v_FIELD_ELEMENTS_IN_VECTOR
-                  }
-                  <:
-                  Core.Ops.Range.t_Range usize)
-              <:
-              Core.Ops.Range.t_Range usize)
-            v
-            (fun v i ->
-                let v:t_PortableVector = v in
-                let i:usize = i in
-                {
-                  v with
-                  f_elements
-                  =
-                  Rust_primitives.Hax.Monomorphized_update_at.update_at_usize v.f_elements
-                    i
-                    (Libcrux_ml_kem.Arithmetic.barrett_reduce (v.f_elements.[ i ] <: i32) <: i32)
-                  <:
-                  t_Array i32 (sz 8)
-                }
-                <:
-                t_PortableVector)
-        in
-        v);
+    f_barrett_reduce = (fun (v: t_PortableVector) -> barrett_reduce v);
     f_montgomery_reduce_pre = (fun (v: t_PortableVector) -> true);
     f_montgomery_reduce_post = (fun (v: t_PortableVector) (out: t_PortableVector) -> true);
-    f_montgomery_reduce
-    =
-    fun (v: t_PortableVector) ->
-      let v:t_PortableVector =
-        Core.Iter.Traits.Iterator.f_fold (Core.Iter.Traits.Collect.f_into_iter ({
-                  Core.Ops.Range.f_start = sz 0;
-                  Core.Ops.Range.f_end = Libcrux_ml_kem.Simd.Simd_trait.v_FIELD_ELEMENTS_IN_VECTOR
-                }
-                <:
-                Core.Ops.Range.t_Range usize)
-            <:
-            Core.Ops.Range.t_Range usize)
-          v
-          (fun v i ->
-              let v:t_PortableVector = v in
-              let i:usize = i in
-              {
-                v with
-                f_elements
-                =
-                Rust_primitives.Hax.Monomorphized_update_at.update_at_usize v.f_elements
-                  i
-                  (Libcrux_ml_kem.Arithmetic.montgomery_reduce (v.f_elements.[ i ] <: i32) <: i32)
-                <:
-                t_Array i32 (sz 8)
-              }
-              <:
-              t_PortableVector)
-      in
-      v
-  }
-
-[@@ FStar.Tactics.Typeclasses.tcinstance]
-let impl_4: Libcrux_ml_kem.Simd.Simd_trait.t_CompressionOperations t_PortableVector =
-  {
+    f_montgomery_reduce = (fun (v: t_PortableVector) -> montgomery_reduce v);
     f_compress_1_pre = (fun (v: t_PortableVector) -> true);
     f_compress_1_post = (fun (v: t_PortableVector) (out: t_PortableVector) -> true);
-    f_compress_1_
-    =
-    (fun (v: t_PortableVector) ->
-        let v:t_PortableVector =
-          Core.Iter.Traits.Iterator.f_fold (Core.Iter.Traits.Collect.f_into_iter ({
-                    Core.Ops.Range.f_start = sz 0;
-                    Core.Ops.Range.f_end = Libcrux_ml_kem.Simd.Simd_trait.v_FIELD_ELEMENTS_IN_VECTOR
-                  }
-                  <:
-                  Core.Ops.Range.t_Range usize)
-              <:
-              Core.Ops.Range.t_Range usize)
-            v
-            (fun v i ->
-                let v:t_PortableVector = v in
-                let i:usize = i in
-                {
-                  v with
-                  f_elements
-                  =
-                  Rust_primitives.Hax.Monomorphized_update_at.update_at_usize v.f_elements
-                    i
-                    (cast (Libcrux_ml_kem.Compress.compress_message_coefficient (cast (v.f_elements.[
-                                    i ]
-                                  <:
-                                  i32)
-                              <:
-                              u16)
-                          <:
-                          u8)
-                      <:
-                      i32)
-                  <:
-                  t_Array i32 (sz 8)
-                }
-                <:
-                t_PortableVector)
-        in
-        v);
+    f_compress_1_ = (fun (v: t_PortableVector) -> compress_1_ v);
     f_compress_pre = (fun (coefficient_bits: u8) (v: t_PortableVector) -> true);
     f_compress_post
     =
     (fun (coefficient_bits: u8) (v: t_PortableVector) (out: t_PortableVector) -> true);
-    f_compress
-    =
-    fun (coefficient_bits: u8) (v: t_PortableVector) ->
-      let v:t_PortableVector =
-        Core.Iter.Traits.Iterator.f_fold (Core.Iter.Traits.Collect.f_into_iter ({
-                  Core.Ops.Range.f_start = sz 0;
-                  Core.Ops.Range.f_end = Libcrux_ml_kem.Simd.Simd_trait.v_FIELD_ELEMENTS_IN_VECTOR
-                }
-                <:
-                Core.Ops.Range.t_Range usize)
-            <:
-            Core.Ops.Range.t_Range usize)
-          v
-          (fun v i ->
-              let v:t_PortableVector = v in
-              let i:usize = i in
-              {
-                v with
-                f_elements
-                =
-                Rust_primitives.Hax.Monomorphized_update_at.update_at_usize v.f_elements
-                  i
-                  (Libcrux_ml_kem.Compress.compress_ciphertext_coefficient coefficient_bits
-                      (cast (v.f_elements.[ i ] <: i32) <: u16)
-                    <:
-                    i32)
-                <:
-                t_Array i32 (sz 8)
-              }
-              <:
-              t_PortableVector)
-      in
-      v
-  }
-
-[@@ FStar.Tactics.Typeclasses.tcinstance]
-let impl_5: Libcrux_ml_kem.Simd.Simd_trait.t_NTTOperations t_PortableVector =
-  {
-    f_ntt_layer_1_step_pre = (fun (v: t_PortableVector) (zeta1: i32) (zeta2: i32) -> true);
+    f_compress = (fun (coefficient_bits: u8) (v: t_PortableVector) -> compress coefficient_bits v);
+    f_ntt_layer_1_step_pre = (fun (a: t_PortableVector) (zeta1: i32) (zeta2: i32) -> true);
     f_ntt_layer_1_step_post
     =
-    (fun (v: t_PortableVector) (zeta1: i32) (zeta2: i32) (out: t_PortableVector) -> true);
+    (fun (a: t_PortableVector) (zeta1: i32) (zeta2: i32) (out: t_PortableVector) -> true);
     f_ntt_layer_1_step
     =
-    (fun (v: t_PortableVector) (zeta1: i32) (zeta2: i32) ->
-        let t:i32 =
-          Libcrux_ml_kem.Arithmetic.montgomery_multiply_fe_by_fer (v.f_elements.[ sz 2 ] <: i32)
-            zeta1
-        in
-        let v:t_PortableVector =
-          {
-            v with
-            f_elements
-            =
-            Rust_primitives.Hax.Monomorphized_update_at.update_at_usize v.f_elements
-              (sz 2)
-              ((v.f_elements.[ sz 0 ] <: i32) -! t <: i32)
-          }
-          <:
-          t_PortableVector
-        in
-        let v:t_PortableVector =
-          {
-            v with
-            f_elements
-            =
-            Rust_primitives.Hax.Monomorphized_update_at.update_at_usize v.f_elements
-              (sz 0)
-              ((v.f_elements.[ sz 0 ] <: i32) +! t <: i32)
-          }
-          <:
-          t_PortableVector
-        in
-        let t:i32 =
-          Libcrux_ml_kem.Arithmetic.montgomery_multiply_fe_by_fer (v.f_elements.[ sz 3 ] <: i32)
-            zeta1
-        in
-        let v:t_PortableVector =
-          {
-            v with
-            f_elements
-            =
-            Rust_primitives.Hax.Monomorphized_update_at.update_at_usize v.f_elements
-              (sz 3)
-              ((v.f_elements.[ sz 1 ] <: i32) -! t <: i32)
-          }
-          <:
-          t_PortableVector
-        in
-        let v:t_PortableVector =
-          {
-            v with
-            f_elements
-            =
-            Rust_primitives.Hax.Monomorphized_update_at.update_at_usize v.f_elements
-              (sz 1)
-              ((v.f_elements.[ sz 1 ] <: i32) +! t <: i32)
-          }
-          <:
-          t_PortableVector
-        in
-        let t:i32 =
-          Libcrux_ml_kem.Arithmetic.montgomery_multiply_fe_by_fer (v.f_elements.[ sz 6 ] <: i32)
-            zeta2
-        in
-        let v:t_PortableVector =
-          {
-            v with
-            f_elements
-            =
-            Rust_primitives.Hax.Monomorphized_update_at.update_at_usize v.f_elements
-              (sz 6)
-              ((v.f_elements.[ sz 4 ] <: i32) -! t <: i32)
-          }
-          <:
-          t_PortableVector
-        in
-        let v:t_PortableVector =
-          {
-            v with
-            f_elements
-            =
-            Rust_primitives.Hax.Monomorphized_update_at.update_at_usize v.f_elements
-              (sz 4)
-              ((v.f_elements.[ sz 4 ] <: i32) +! t <: i32)
-          }
-          <:
-          t_PortableVector
-        in
-        let t:i32 =
-          Libcrux_ml_kem.Arithmetic.montgomery_multiply_fe_by_fer (v.f_elements.[ sz 7 ] <: i32)
-            zeta2
-        in
-        let v:t_PortableVector =
-          {
-            v with
-            f_elements
-            =
-            Rust_primitives.Hax.Monomorphized_update_at.update_at_usize v.f_elements
-              (sz 7)
-              ((v.f_elements.[ sz 5 ] <: i32) -! t <: i32)
-          }
-          <:
-          t_PortableVector
-        in
-        let v:t_PortableVector =
-          {
-            v with
-            f_elements
-            =
-            Rust_primitives.Hax.Monomorphized_update_at.update_at_usize v.f_elements
-              (sz 5)
-              ((v.f_elements.[ sz 5 ] <: i32) +! t <: i32)
-          }
-          <:
-          t_PortableVector
-        in
-        v);
-    f_ntt_layer_2_step_pre = (fun (v: t_PortableVector) (zeta: i32) -> true);
+    (fun (a: t_PortableVector) (zeta1: i32) (zeta2: i32) -> ntt_layer_1_step a zeta1 zeta2);
+    f_ntt_layer_2_step_pre = (fun (a: t_PortableVector) (zeta: i32) -> true);
     f_ntt_layer_2_step_post
     =
-    (fun (v: t_PortableVector) (zeta: i32) (out: t_PortableVector) -> true);
-    f_ntt_layer_2_step
-    =
-    (fun (v: t_PortableVector) (zeta: i32) ->
-        let t:i32 =
-          Libcrux_ml_kem.Arithmetic.montgomery_multiply_fe_by_fer (v.f_elements.[ sz 4 ] <: i32)
-            zeta
-        in
-        let v:t_PortableVector =
-          {
-            v with
-            f_elements
-            =
-            Rust_primitives.Hax.Monomorphized_update_at.update_at_usize v.f_elements
-              (sz 4)
-              ((v.f_elements.[ sz 0 ] <: i32) -! t <: i32)
-          }
-          <:
-          t_PortableVector
-        in
-        let v:t_PortableVector =
-          {
-            v with
-            f_elements
-            =
-            Rust_primitives.Hax.Monomorphized_update_at.update_at_usize v.f_elements
-              (sz 0)
-              ((v.f_elements.[ sz 0 ] <: i32) +! t <: i32)
-          }
-          <:
-          t_PortableVector
-        in
-        let t:i32 =
-          Libcrux_ml_kem.Arithmetic.montgomery_multiply_fe_by_fer (v.f_elements.[ sz 5 ] <: i32)
-            zeta
-        in
-        let v:t_PortableVector =
-          {
-            v with
-            f_elements
-            =
-            Rust_primitives.Hax.Monomorphized_update_at.update_at_usize v.f_elements
-              (sz 5)
-              ((v.f_elements.[ sz 1 ] <: i32) -! t <: i32)
-          }
-          <:
-          t_PortableVector
-        in
-        let v:t_PortableVector =
-          {
-            v with
-            f_elements
-            =
-            Rust_primitives.Hax.Monomorphized_update_at.update_at_usize v.f_elements
-              (sz 1)
-              ((v.f_elements.[ sz 1 ] <: i32) +! t <: i32)
-          }
-          <:
-          t_PortableVector
-        in
-        let t:i32 =
-          Libcrux_ml_kem.Arithmetic.montgomery_multiply_fe_by_fer (v.f_elements.[ sz 6 ] <: i32)
-            zeta
-        in
-        let v:t_PortableVector =
-          {
-            v with
-            f_elements
-            =
-            Rust_primitives.Hax.Monomorphized_update_at.update_at_usize v.f_elements
-              (sz 6)
-              ((v.f_elements.[ sz 2 ] <: i32) -! t <: i32)
-          }
-          <:
-          t_PortableVector
-        in
-        let v:t_PortableVector =
-          {
-            v with
-            f_elements
-            =
-            Rust_primitives.Hax.Monomorphized_update_at.update_at_usize v.f_elements
-              (sz 2)
-              ((v.f_elements.[ sz 2 ] <: i32) +! t <: i32)
-          }
-          <:
-          t_PortableVector
-        in
-        let t:i32 =
-          Libcrux_ml_kem.Arithmetic.montgomery_multiply_fe_by_fer (v.f_elements.[ sz 7 ] <: i32)
-            zeta
-        in
-        let v:t_PortableVector =
-          {
-            v with
-            f_elements
-            =
-            Rust_primitives.Hax.Monomorphized_update_at.update_at_usize v.f_elements
-              (sz 7)
-              ((v.f_elements.[ sz 3 ] <: i32) -! t <: i32)
-          }
-          <:
-          t_PortableVector
-        in
-        let v:t_PortableVector =
-          {
-            v with
-            f_elements
-            =
-            Rust_primitives.Hax.Monomorphized_update_at.update_at_usize v.f_elements
-              (sz 3)
-              ((v.f_elements.[ sz 3 ] <: i32) +! t <: i32)
-          }
-          <:
-          t_PortableVector
-        in
-        v);
-    f_inv_ntt_layer_1_step_pre = (fun (v: t_PortableVector) (zeta1: i32) (zeta2: i32) -> true);
+    (fun (a: t_PortableVector) (zeta: i32) (out: t_PortableVector) -> true);
+    f_ntt_layer_2_step = (fun (a: t_PortableVector) (zeta: i32) -> ntt_layer_2_step a zeta);
+    f_inv_ntt_layer_1_step_pre = (fun (a: t_PortableVector) (zeta1: i32) (zeta2: i32) -> true);
     f_inv_ntt_layer_1_step_post
     =
-    (fun (v: t_PortableVector) (zeta1: i32) (zeta2: i32) (out: t_PortableVector) -> true);
+    (fun (a: t_PortableVector) (zeta1: i32) (zeta2: i32) (out: t_PortableVector) -> true);
     f_inv_ntt_layer_1_step
     =
-    (fun (v: t_PortableVector) (zeta1: i32) (zeta2: i32) ->
-        let a_minus_b:i32 = (v.f_elements.[ sz 2 ] <: i32) -! (v.f_elements.[ sz 0 ] <: i32) in
-        let v:t_PortableVector =
-          {
-            v with
-            f_elements
-            =
-            Rust_primitives.Hax.Monomorphized_update_at.update_at_usize v.f_elements
-              (sz 0)
-              ((v.f_elements.[ sz 0 ] <: i32) +! (v.f_elements.[ sz 2 ] <: i32) <: i32)
-          }
-          <:
-          t_PortableVector
-        in
-        let v:t_PortableVector =
-          {
-            v with
-            f_elements
-            =
-            Rust_primitives.Hax.Monomorphized_update_at.update_at_usize v.f_elements
-              (sz 2)
-              (Libcrux_ml_kem.Arithmetic.montgomery_multiply_fe_by_fer a_minus_b zeta1 <: i32)
-          }
-          <:
-          t_PortableVector
-        in
-        let a_minus_b:i32 = (v.f_elements.[ sz 3 ] <: i32) -! (v.f_elements.[ sz 1 ] <: i32) in
-        let v:t_PortableVector =
-          {
-            v with
-            f_elements
-            =
-            Rust_primitives.Hax.Monomorphized_update_at.update_at_usize v.f_elements
-              (sz 1)
-              ((v.f_elements.[ sz 1 ] <: i32) +! (v.f_elements.[ sz 3 ] <: i32) <: i32)
-          }
-          <:
-          t_PortableVector
-        in
-        let v:t_PortableVector =
-          {
-            v with
-            f_elements
-            =
-            Rust_primitives.Hax.Monomorphized_update_at.update_at_usize v.f_elements
-              (sz 3)
-              (Libcrux_ml_kem.Arithmetic.montgomery_multiply_fe_by_fer a_minus_b zeta1 <: i32)
-          }
-          <:
-          t_PortableVector
-        in
-        let a_minus_b:i32 = (v.f_elements.[ sz 6 ] <: i32) -! (v.f_elements.[ sz 4 ] <: i32) in
-        let v:t_PortableVector =
-          {
-            v with
-            f_elements
-            =
-            Rust_primitives.Hax.Monomorphized_update_at.update_at_usize v.f_elements
-              (sz 4)
-              ((v.f_elements.[ sz 4 ] <: i32) +! (v.f_elements.[ sz 6 ] <: i32) <: i32)
-          }
-          <:
-          t_PortableVector
-        in
-        let v:t_PortableVector =
-          {
-            v with
-            f_elements
-            =
-            Rust_primitives.Hax.Monomorphized_update_at.update_at_usize v.f_elements
-              (sz 6)
-              (Libcrux_ml_kem.Arithmetic.montgomery_multiply_fe_by_fer a_minus_b zeta2 <: i32)
-          }
-          <:
-          t_PortableVector
-        in
-        let a_minus_b:i32 = (v.f_elements.[ sz 7 ] <: i32) -! (v.f_elements.[ sz 5 ] <: i32) in
-        let v:t_PortableVector =
-          {
-            v with
-            f_elements
-            =
-            Rust_primitives.Hax.Monomorphized_update_at.update_at_usize v.f_elements
-              (sz 5)
-              ((v.f_elements.[ sz 5 ] <: i32) +! (v.f_elements.[ sz 7 ] <: i32) <: i32)
-          }
-          <:
-          t_PortableVector
-        in
-        let v:t_PortableVector =
-          {
-            v with
-            f_elements
-            =
-            Rust_primitives.Hax.Monomorphized_update_at.update_at_usize v.f_elements
-              (sz 7)
-              (Libcrux_ml_kem.Arithmetic.montgomery_multiply_fe_by_fer a_minus_b zeta2 <: i32)
-          }
-          <:
-          t_PortableVector
-        in
-        v);
-    f_inv_ntt_layer_2_step_pre = (fun (v: t_PortableVector) (zeta: i32) -> true);
+    (fun (a: t_PortableVector) (zeta1: i32) (zeta2: i32) -> inv_ntt_layer_1_step a zeta1 zeta2);
+    f_inv_ntt_layer_2_step_pre = (fun (a: t_PortableVector) (zeta: i32) -> true);
     f_inv_ntt_layer_2_step_post
     =
-    (fun (v: t_PortableVector) (zeta: i32) (out: t_PortableVector) -> true);
-    f_inv_ntt_layer_2_step
-    =
-    (fun (v: t_PortableVector) (zeta: i32) ->
-        let a_minus_b:i32 = (v.f_elements.[ sz 4 ] <: i32) -! (v.f_elements.[ sz 0 ] <: i32) in
-        let v:t_PortableVector =
-          {
-            v with
-            f_elements
-            =
-            Rust_primitives.Hax.Monomorphized_update_at.update_at_usize v.f_elements
-              (sz 0)
-              ((v.f_elements.[ sz 0 ] <: i32) +! (v.f_elements.[ sz 4 ] <: i32) <: i32)
-          }
-          <:
-          t_PortableVector
-        in
-        let v:t_PortableVector =
-          {
-            v with
-            f_elements
-            =
-            Rust_primitives.Hax.Monomorphized_update_at.update_at_usize v.f_elements
-              (sz 4)
-              (Libcrux_ml_kem.Arithmetic.montgomery_multiply_fe_by_fer a_minus_b zeta <: i32)
-          }
-          <:
-          t_PortableVector
-        in
-        let a_minus_b:i32 = (v.f_elements.[ sz 5 ] <: i32) -! (v.f_elements.[ sz 1 ] <: i32) in
-        let v:t_PortableVector =
-          {
-            v with
-            f_elements
-            =
-            Rust_primitives.Hax.Monomorphized_update_at.update_at_usize v.f_elements
-              (sz 1)
-              ((v.f_elements.[ sz 1 ] <: i32) +! (v.f_elements.[ sz 5 ] <: i32) <: i32)
-          }
-          <:
-          t_PortableVector
-        in
-        let v:t_PortableVector =
-          {
-            v with
-            f_elements
-            =
-            Rust_primitives.Hax.Monomorphized_update_at.update_at_usize v.f_elements
-              (sz 5)
-              (Libcrux_ml_kem.Arithmetic.montgomery_multiply_fe_by_fer a_minus_b zeta <: i32)
-          }
-          <:
-          t_PortableVector
-        in
-        let a_minus_b:i32 = (v.f_elements.[ sz 6 ] <: i32) -! (v.f_elements.[ sz 2 ] <: i32) in
-        let v:t_PortableVector =
-          {
-            v with
-            f_elements
-            =
-            Rust_primitives.Hax.Monomorphized_update_at.update_at_usize v.f_elements
-              (sz 2)
-              ((v.f_elements.[ sz 2 ] <: i32) +! (v.f_elements.[ sz 6 ] <: i32) <: i32)
-          }
-          <:
-          t_PortableVector
-        in
-        let v:t_PortableVector =
-          {
-            v with
-            f_elements
-            =
-            Rust_primitives.Hax.Monomorphized_update_at.update_at_usize v.f_elements
-              (sz 6)
-              (Libcrux_ml_kem.Arithmetic.montgomery_multiply_fe_by_fer a_minus_b zeta <: i32)
-          }
-          <:
-          t_PortableVector
-        in
-        let a_minus_b:i32 = (v.f_elements.[ sz 7 ] <: i32) -! (v.f_elements.[ sz 3 ] <: i32) in
-        let v:t_PortableVector =
-          {
-            v with
-            f_elements
-            =
-            Rust_primitives.Hax.Monomorphized_update_at.update_at_usize v.f_elements
-              (sz 3)
-              ((v.f_elements.[ sz 3 ] <: i32) +! (v.f_elements.[ sz 7 ] <: i32) <: i32)
-          }
-          <:
-          t_PortableVector
-        in
-        let v:t_PortableVector =
-          {
-            v with
-            f_elements
-            =
-            Rust_primitives.Hax.Monomorphized_update_at.update_at_usize v.f_elements
-              (sz 7)
-              (Libcrux_ml_kem.Arithmetic.montgomery_multiply_fe_by_fer a_minus_b zeta <: i32)
-          }
-          <:
-          t_PortableVector
-        in
-        v);
+    (fun (a: t_PortableVector) (zeta: i32) (out: t_PortableVector) -> true);
+    f_inv_ntt_layer_2_step = (fun (a: t_PortableVector) (zeta: i32) -> inv_ntt_layer_2_step a zeta);
     f_ntt_multiply_pre
     =
     (fun (lhs: t_PortableVector) (rhs: t_PortableVector) (zeta0: i32) (zeta1: i32) -> true);
@@ -923,230 +198,47 @@ let impl_5: Libcrux_ml_kem.Simd.Simd_trait.t_NTTOperations t_PortableVector =
         (rhs: t_PortableVector)
         (zeta0: i32)
         (zeta1: i32)
-        (out1: t_PortableVector)
+        (out: t_PortableVector)
         ->
         true);
     f_ntt_multiply
     =
-    fun (lhs: t_PortableVector) (rhs: t_PortableVector) (zeta0: i32) (zeta1: i32) ->
-      let out:t_PortableVector = Libcrux_ml_kem.Simd.Simd_trait.f_ZERO () in
-      let product:(i32 & i32) =
-        Libcrux_ml_kem.Arithmetic.ntt_multiply_binomials ((lhs.f_elements.[ sz 0 ] <: i32),
-            (lhs.f_elements.[ sz 1 ] <: i32)
-            <:
-            (i32 & i32))
-          ((rhs.f_elements.[ sz 0 ] <: i32), (rhs.f_elements.[ sz 1 ] <: i32) <: (i32 & i32))
-          zeta0
-      in
-      let out:t_PortableVector =
-        {
-          out with
-          f_elements
-          =
-          Rust_primitives.Hax.Monomorphized_update_at.update_at_usize out.f_elements
-            (sz 0)
-            product._1
-        }
-        <:
-        t_PortableVector
-      in
-      let out:t_PortableVector =
-        {
-          out with
-          f_elements
-          =
-          Rust_primitives.Hax.Monomorphized_update_at.update_at_usize out.f_elements
-            (sz 1)
-            product._2
-        }
-        <:
-        t_PortableVector
-      in
-      let product:(i32 & i32) =
-        Libcrux_ml_kem.Arithmetic.ntt_multiply_binomials ((lhs.f_elements.[ sz 2 ] <: i32),
-            (lhs.f_elements.[ sz 3 ] <: i32)
-            <:
-            (i32 & i32))
-          ((rhs.f_elements.[ sz 2 ] <: i32), (rhs.f_elements.[ sz 3 ] <: i32) <: (i32 & i32))
-          (Core.Ops.Arith.Neg.neg zeta0 <: i32)
-      in
-      let out:t_PortableVector =
-        {
-          out with
-          f_elements
-          =
-          Rust_primitives.Hax.Monomorphized_update_at.update_at_usize out.f_elements
-            (sz 2)
-            product._1
-        }
-        <:
-        t_PortableVector
-      in
-      let out:t_PortableVector =
-        {
-          out with
-          f_elements
-          =
-          Rust_primitives.Hax.Monomorphized_update_at.update_at_usize out.f_elements
-            (sz 3)
-            product._2
-        }
-        <:
-        t_PortableVector
-      in
-      let product:(i32 & i32) =
-        Libcrux_ml_kem.Arithmetic.ntt_multiply_binomials ((lhs.f_elements.[ sz 4 ] <: i32),
-            (lhs.f_elements.[ sz 5 ] <: i32)
-            <:
-            (i32 & i32))
-          ((rhs.f_elements.[ sz 4 ] <: i32), (rhs.f_elements.[ sz 5 ] <: i32) <: (i32 & i32))
-          zeta1
-      in
-      let out:t_PortableVector =
-        {
-          out with
-          f_elements
-          =
-          Rust_primitives.Hax.Monomorphized_update_at.update_at_usize out.f_elements
-            (sz 4)
-            product._1
-        }
-        <:
-        t_PortableVector
-      in
-      let out:t_PortableVector =
-        {
-          out with
-          f_elements
-          =
-          Rust_primitives.Hax.Monomorphized_update_at.update_at_usize out.f_elements
-            (sz 5)
-            product._2
-        }
-        <:
-        t_PortableVector
-      in
-      let product:(i32 & i32) =
-        Libcrux_ml_kem.Arithmetic.ntt_multiply_binomials ((lhs.f_elements.[ sz 6 ] <: i32),
-            (lhs.f_elements.[ sz 7 ] <: i32)
-            <:
-            (i32 & i32))
-          ((rhs.f_elements.[ sz 6 ] <: i32), (rhs.f_elements.[ sz 7 ] <: i32) <: (i32 & i32))
-          (Core.Ops.Arith.Neg.neg zeta1 <: i32)
-      in
-      let out:t_PortableVector =
-        {
-          out with
-          f_elements
-          =
-          Rust_primitives.Hax.Monomorphized_update_at.update_at_usize out.f_elements
-            (sz 6)
-            product._1
-        }
-        <:
-        t_PortableVector
-      in
-      let out:t_PortableVector =
-        {
-          out with
-          f_elements
-          =
-          Rust_primitives.Hax.Monomorphized_update_at.update_at_usize out.f_elements
-            (sz 7)
-            product._2
-        }
-        <:
-        t_PortableVector
-      in
-      out
-  }
-
-val deserialize_10___ (bytes: t_Slice u8)
-    : Prims.Pure t_PortableVector Prims.l_True (fun _ -> Prims.l_True)
-
-val deserialize_11___ (bytes: t_Slice u8)
-    : Prims.Pure t_PortableVector Prims.l_True (fun _ -> Prims.l_True)
-
-val deserialize_12___ (bytes: t_Slice u8)
-    : Prims.Pure t_PortableVector Prims.l_True (fun _ -> Prims.l_True)
-
-val deserialize_1___ (v: u8) : Prims.Pure t_PortableVector Prims.l_True (fun _ -> Prims.l_True)
-
-val deserialize_4___ (bytes: t_Slice u8)
-    : Prims.Pure t_PortableVector Prims.l_True (fun _ -> Prims.l_True)
-
-val deserialize_5___ (bytes: t_Slice u8)
-    : Prims.Pure t_PortableVector Prims.l_True (fun _ -> Prims.l_True)
-
-val serialize_10___ (v: t_PortableVector)
-    : Prims.Pure (t_Array u8 (sz 10)) Prims.l_True (fun _ -> Prims.l_True)
-
-val serialize_11___ (v: t_PortableVector)
-    : Prims.Pure (t_Array u8 (sz 11)) Prims.l_True (fun _ -> Prims.l_True)
-
-val serialize_12___ (v: t_PortableVector)
-    : Prims.Pure (t_Array u8 (sz 12)) Prims.l_True (fun _ -> Prims.l_True)
-
-val serialize_1___ (v: t_PortableVector) : Prims.Pure u8 Prims.l_True (fun _ -> Prims.l_True)
-
-val serialize_4___ (v: t_PortableVector)
-    : Prims.Pure (t_Array u8 (sz 4)) Prims.l_True (fun _ -> Prims.l_True)
-
-val serialize_5___ (v: t_PortableVector)
-    : Prims.Pure (t_Array u8 (sz 5)) Prims.l_True (fun _ -> Prims.l_True)
-
-[@@ FStar.Tactics.Typeclasses.tcinstance]
-let impl_6: Libcrux_ml_kem.Simd.Simd_trait.t_SerializeOperations t_PortableVector =
-  {
+    (fun (lhs: t_PortableVector) (rhs: t_PortableVector) (zeta0: i32) (zeta1: i32) ->
+        ntt_multiply lhs rhs zeta0 zeta1);
     f_serialize_1_pre = (fun (a: t_PortableVector) -> true);
     f_serialize_1_post = (fun (a: t_PortableVector) (out: u8) -> true);
-    f_serialize_1_ = (fun (a: t_PortableVector) -> serialize_1___ a);
+    f_serialize_1_ = (fun (a: t_PortableVector) -> serialize_1_ a);
     f_deserialize_1_pre = (fun (a: u8) -> true);
     f_deserialize_1_post = (fun (a: u8) (out: t_PortableVector) -> true);
-    f_deserialize_1_ = (fun (a: u8) -> deserialize_1___ a);
+    f_deserialize_1_ = (fun (a: u8) -> deserialize_1_ a);
     f_serialize_4_pre = (fun (a: t_PortableVector) -> true);
     f_serialize_4_post = (fun (a: t_PortableVector) (out: t_Array u8 (sz 4)) -> true);
-    f_serialize_4_ = (fun (a: t_PortableVector) -> serialize_4___ a);
+    f_serialize_4_ = (fun (a: t_PortableVector) -> serialize_4_ a);
     f_deserialize_4_pre = (fun (a: t_Slice u8) -> true);
     f_deserialize_4_post = (fun (a: t_Slice u8) (out: t_PortableVector) -> true);
-    f_deserialize_4_ = (fun (a: t_Slice u8) -> deserialize_4___ a);
+    f_deserialize_4_ = (fun (a: t_Slice u8) -> deserialize_4_ a);
     f_serialize_5_pre = (fun (a: t_PortableVector) -> true);
     f_serialize_5_post = (fun (a: t_PortableVector) (out: t_Array u8 (sz 5)) -> true);
-    f_serialize_5_ = (fun (a: t_PortableVector) -> serialize_5___ a);
+    f_serialize_5_ = (fun (a: t_PortableVector) -> serialize_5_ a);
     f_deserialize_5_pre = (fun (a: t_Slice u8) -> true);
     f_deserialize_5_post = (fun (a: t_Slice u8) (out: t_PortableVector) -> true);
-    f_deserialize_5_ = (fun (a: t_Slice u8) -> deserialize_5___ a);
+    f_deserialize_5_ = (fun (a: t_Slice u8) -> deserialize_5_ a);
     f_serialize_10_pre = (fun (a: t_PortableVector) -> true);
     f_serialize_10_post = (fun (a: t_PortableVector) (out: t_Array u8 (sz 10)) -> true);
-    f_serialize_10_ = (fun (a: t_PortableVector) -> serialize_10___ a);
+    f_serialize_10_ = (fun (a: t_PortableVector) -> serialize_10_ a);
     f_deserialize_10_pre = (fun (a: t_Slice u8) -> true);
     f_deserialize_10_post = (fun (a: t_Slice u8) (out: t_PortableVector) -> true);
-    f_deserialize_10_ = (fun (a: t_Slice u8) -> deserialize_10___ a);
+    f_deserialize_10_ = (fun (a: t_Slice u8) -> deserialize_10_ a);
     f_serialize_11_pre = (fun (a: t_PortableVector) -> true);
     f_serialize_11_post = (fun (a: t_PortableVector) (out: t_Array u8 (sz 11)) -> true);
-    f_serialize_11_ = (fun (a: t_PortableVector) -> serialize_11___ a);
+    f_serialize_11_ = (fun (a: t_PortableVector) -> serialize_11_ a);
     f_deserialize_11_pre = (fun (a: t_Slice u8) -> true);
     f_deserialize_11_post = (fun (a: t_Slice u8) (out: t_PortableVector) -> true);
-    f_deserialize_11_ = (fun (a: t_Slice u8) -> deserialize_11___ a);
+    f_deserialize_11_ = (fun (a: t_Slice u8) -> deserialize_11_ a);
     f_serialize_12_pre = (fun (a: t_PortableVector) -> true);
     f_serialize_12_post = (fun (a: t_PortableVector) (out: t_Array u8 (sz 12)) -> true);
-    f_serialize_12_ = (fun (a: t_PortableVector) -> serialize_12___ a);
+    f_serialize_12_ = (fun (a: t_PortableVector) -> serialize_12_ a);
     f_deserialize_12_pre = (fun (a: t_Slice u8) -> true);
     f_deserialize_12_post = (fun (a: t_Slice u8) (out: t_PortableVector) -> true);
-    f_deserialize_12_ = fun (a: t_Slice u8) -> deserialize_12___ a
-  }
-
-[@@ FStar.Tactics.Typeclasses.tcinstance]
-let impl_7: Libcrux_ml_kem.Simd.Simd_trait.t_Operations t_PortableVector =
-  {
-    _super_16550665238208597986 = FStar.Tactics.Typeclasses.solve;
-    _super_9181983936900423582 = FStar.Tactics.Typeclasses.solve;
-    _super_11057338832248834886 = FStar.Tactics.Typeclasses.solve;
-    _super_5739476159407468282 = FStar.Tactics.Typeclasses.solve;
-    _super_13298396156660513588 = FStar.Tactics.Typeclasses.solve;
-    _super_1988623142765322925 = FStar.Tactics.Typeclasses.solve;
-    _super_18188678553863793517 = FStar.Tactics.Typeclasses.solve;
-    _super_957087622381469234 = FStar.Tactics.Typeclasses.solve;
-    _super_2101570567305961368 = FStar.Tactics.Typeclasses.solve;
-    __marker_trait = ()
+    f_deserialize_12_ = fun (a: t_Slice u8) -> deserialize_12_ a
   }
