libcrux-ml-kem/proofs/fstar/extraction/Libcrux_ml_kem.Polynomial.fst
@@ -3,38 +3,6 @@ module Libcrux_ml_kem.Polynomial
 open Core
 open FStar.Mul
 
-let ntt_layer_7_int_vec_step (a b: Libcrux_ml_kem.Simd.Portable.t_PortableVector) =
-  let t:Libcrux_ml_kem.Simd.Portable.t_PortableVector =
-    Libcrux_ml_kem.Simd.Simd_trait.f_multiply_by_constant b (-1600l)
-  in
-  let b:Libcrux_ml_kem.Simd.Portable.t_PortableVector = Libcrux_ml_kem.Simd.Simd_trait.f_sub a t in
-  let a:Libcrux_ml_kem.Simd.Portable.t_PortableVector = Libcrux_ml_kem.Simd.Simd_trait.f_add a t in
-  a, b
-  <:
-  (Libcrux_ml_kem.Simd.Portable.t_PortableVector & Libcrux_ml_kem.Simd.Portable.t_PortableVector)
-
-let inv_ntt_layer_int_vec_step (a b: Libcrux_ml_kem.Simd.Portable.t_PortableVector) (zeta_r: i32) =
-  let a_minus_b:Libcrux_ml_kem.Simd.Portable.t_PortableVector =
-    Libcrux_ml_kem.Simd.Simd_trait.f_sub b a
-  in
-  let a:Libcrux_ml_kem.Simd.Portable.t_PortableVector = Libcrux_ml_kem.Simd.Simd_trait.f_add a b in
-  let b:Libcrux_ml_kem.Simd.Portable.t_PortableVector =
-    Libcrux_ml_kem.Simd.Simd_trait.f_montgomery_multiply_fe_by_fer a_minus_b zeta_r
-  in
-  a, b
-  <:
-  (Libcrux_ml_kem.Simd.Portable.t_PortableVector & Libcrux_ml_kem.Simd.Portable.t_PortableVector)
-
-let ntt_layer_int_vec_step (a b: Libcrux_ml_kem.Simd.Portable.t_PortableVector) (zeta_r: i32) =
-  let t:Libcrux_ml_kem.Simd.Portable.t_PortableVector =
-    Libcrux_ml_kem.Simd.Simd_trait.f_montgomery_multiply_fe_by_fer b zeta_r
-  in
-  let b:Libcrux_ml_kem.Simd.Portable.t_PortableVector = Libcrux_ml_kem.Simd.Simd_trait.f_sub a t in
-  let a:Libcrux_ml_kem.Simd.Portable.t_PortableVector = Libcrux_ml_kem.Simd.Simd_trait.f_add a t in
-  a, b
-  <:
-  (Libcrux_ml_kem.Simd.Portable.t_PortableVector & Libcrux_ml_kem.Simd.Portable.t_PortableVector)
-
 let impl__PolynomialRingElement__ZERO (_: Prims.unit) =
   {
     f_coefficients
@@ -274,6 +242,18 @@ let from_i32_array (a: t_Array i32 (sz 256)) =
   in
   result
 
+let inv_ntt_layer_int_vec_step (a b: Libcrux_ml_kem.Simd.Portable.t_PortableVector) (zeta_r: i32) =
+  let a_minus_b:Libcrux_ml_kem.Simd.Portable.t_PortableVector =
+    Libcrux_ml_kem.Simd.Simd_trait.f_sub b a
+  in
+  let a:Libcrux_ml_kem.Simd.Portable.t_PortableVector = Libcrux_ml_kem.Simd.Simd_trait.f_add a b in
+  let b:Libcrux_ml_kem.Simd.Portable.t_PortableVector =
+    Libcrux_ml_kem.Simd.Simd_trait.f_montgomery_multiply_fe_by_fer a_minus_b zeta_r
+  in
+  a, b
+  <:
+  (Libcrux_ml_kem.Simd.Portable.t_PortableVector & Libcrux_ml_kem.Simd.Portable.t_PortableVector)
+
 let invert_ntt_at_layer_1_ (zeta_i: usize) (re: t_PolynomialRingElement) (v__layer: usize) =
   let zeta_i:usize = zeta_i -! sz 1 in
   let re, zeta_i:(t_PolynomialRingElement & usize) =
@@ -511,6 +491,76 @@ let ntt_at_layer_2_
   let hax_temp_output:t_PolynomialRingElement = re in
   zeta_i, hax_temp_output <: (usize & t_PolynomialRingElement)
 
+let ntt_layer_7_int_vec_step (a b: Libcrux_ml_kem.Simd.Portable.t_PortableVector) =
+  let t:Libcrux_ml_kem.Simd.Portable.t_PortableVector =
+    Libcrux_ml_kem.Simd.Simd_trait.f_multiply_by_constant b (-1600l)
+  in
+  let b:Libcrux_ml_kem.Simd.Portable.t_PortableVector = Libcrux_ml_kem.Simd.Simd_trait.f_sub a t in
+  let a:Libcrux_ml_kem.Simd.Portable.t_PortableVector = Libcrux_ml_kem.Simd.Simd_trait.f_add a t in
+  a, b
+  <:
+  (Libcrux_ml_kem.Simd.Portable.t_PortableVector & Libcrux_ml_kem.Simd.Portable.t_PortableVector)
+
+let ntt_at_layer_7_ (re: t_PolynomialRingElement) =
+  let step:usize = v_VECTORS_IN_RING_ELEMENT /! sz 2 in
+  let re:t_PolynomialRingElement =
+    Core.Iter.Traits.Iterator.f_fold (Core.Iter.Traits.Collect.f_into_iter ({
+              Core.Ops.Range.f_start = sz 0;
+              Core.Ops.Range.f_end = step
+            }
+            <:
+            Core.Ops.Range.t_Range usize)
+        <:
+        Core.Ops.Range.t_Range usize)
+      re
+      (fun re j ->
+          let re:t_PolynomialRingElement = re in
+          let j:usize = j in
+          let x, y:(Libcrux_ml_kem.Simd.Portable.t_PortableVector &
+            Libcrux_ml_kem.Simd.Portable.t_PortableVector) =
+            ntt_layer_7_int_vec_step (re.f_coefficients.[ j ]
+                <:
+                Libcrux_ml_kem.Simd.Portable.t_PortableVector)
+              (re.f_coefficients.[ j +! step <: usize ]
+                <:
+                Libcrux_ml_kem.Simd.Portable.t_PortableVector)
+          in
+          let re:t_PolynomialRingElement =
+            {
+              re with
+              f_coefficients
+              =
+              Rust_primitives.Hax.Monomorphized_update_at.update_at_usize re.f_coefficients j x
+            }
+            <:
+            t_PolynomialRingElement
+          in
+          let re:t_PolynomialRingElement =
+            {
+              re with
+              f_coefficients
+              =
+              Rust_primitives.Hax.Monomorphized_update_at.update_at_usize re.f_coefficients
+                (j +! step <: usize)
+                y
+            }
+            <:
+            t_PolynomialRingElement
+          in
+          re)
+  in
+  re
+
+let ntt_layer_int_vec_step (a b: Libcrux_ml_kem.Simd.Portable.t_PortableVector) (zeta_r: i32) =
+  let t:Libcrux_ml_kem.Simd.Portable.t_PortableVector =
+    Libcrux_ml_kem.Simd.Simd_trait.f_montgomery_multiply_fe_by_fer b zeta_r
+  in
+  let b:Libcrux_ml_kem.Simd.Portable.t_PortableVector = Libcrux_ml_kem.Simd.Simd_trait.f_sub a t in
+  let a:Libcrux_ml_kem.Simd.Portable.t_PortableVector = Libcrux_ml_kem.Simd.Simd_trait.f_add a t in
+  a, b
+  <:
+  (Libcrux_ml_kem.Simd.Portable.t_PortableVector & Libcrux_ml_kem.Simd.Portable.t_PortableVector)
+
 let ntt_at_layer_3_plus
       (zeta_i: usize)
       (re: t_PolynomialRingElement)
@@ -601,56 +651,6 @@ let ntt_at_layer_3_plus
   in
   let hax_temp_output:t_PolynomialRingElement = re in
   zeta_i, hax_temp_output <: (usize & t_PolynomialRingElement)
-
-let ntt_at_layer_7_ (re: t_PolynomialRingElement) =
-  let step:usize = v_VECTORS_IN_RING_ELEMENT /! sz 2 in
-  let re:t_PolynomialRingElement =
-    Core.Iter.Traits.Iterator.f_fold (Core.Iter.Traits.Collect.f_into_iter ({
-              Core.Ops.Range.f_start = sz 0;
-              Core.Ops.Range.f_end = step
-            }
-            <:
-            Core.Ops.Range.t_Range usize)
-        <:
-        Core.Ops.Range.t_Range usize)
-      re
-      (fun re j ->
-          let re:t_PolynomialRingElement = re in
-          let j:usize = j in
-          let x, y:(Libcrux_ml_kem.Simd.Portable.t_PortableVector &
-            Libcrux_ml_kem.Simd.Portable.t_PortableVector) =
-            ntt_layer_7_int_vec_step (re.f_coefficients.[ j ]
-                <:
-                Libcrux_ml_kem.Simd.Portable.t_PortableVector)
-              (re.f_coefficients.[ j +! step <: usize ]
-                <:
-                Libcrux_ml_kem.Simd.Portable.t_PortableVector)
-          in
-          let re:t_PolynomialRingElement =
-            {
-              re with
-              f_coefficients
-              =
-              Rust_primitives.Hax.Monomorphized_update_at.update_at_usize re.f_coefficients j x
-            }
-            <:
-            t_PolynomialRingElement
-          in
-          let re:t_PolynomialRingElement =
-            {
-              re with
-              f_coefficients
-              =
-              Rust_primitives.Hax.Monomorphized_update_at.update_at_usize re.f_coefficients
-                (j +! step <: usize)
-                y
-            }
-            <:
-            t_PolynomialRingElement
-          in
-          re)
-  in
-  re
 
 let ntt_multiply (lhs rhs: t_PolynomialRingElement) =
   let out:t_PolynomialRingElement = impl__PolynomialRingElement__ZERO () in
