libcrux-ml-kem/proofs/fstar/extraction/Libcrux_ml_kem.Simd.Simd_trait.fsti
@@ -3,71 +3,6 @@ module Libcrux_ml_kem.Simd.Simd_trait
 open Core
 open FStar.Mul
 
-class t_ArithmeticOperations (v_Self: Type) = {
-  f_add_constant_pre:v_Self -> i32 -> bool;
-  f_add_constant_post:v_Self -> i32 -> v_Self -> bool;
-  f_add_constant:x0: v_Self -> x1: i32
-    -> Prims.Pure v_Self (f_add_constant_pre x0 x1) (fun result -> f_add_constant_post x0 x1 result);
-  f_add_pre:v_Self -> v_Self -> bool;
-  f_add_post:v_Self -> v_Self -> v_Self -> bool;
-  f_add:x0: v_Self -> x1: v_Self
-    -> Prims.Pure v_Self (f_add_pre x0 x1) (fun result -> f_add_post x0 x1 result);
-  f_sub_pre:v_Self -> v_Self -> bool;
-  f_sub_post:v_Self -> v_Self -> v_Self -> bool;
-  f_sub:x0: v_Self -> x1: v_Self
-    -> Prims.Pure v_Self (f_sub_pre x0 x1) (fun result -> f_sub_post x0 x1 result);
-  f_multiply_by_constant_pre:v_Self -> i32 -> bool;
-  f_multiply_by_constant_post:v_Self -> i32 -> v_Self -> bool;
-  f_multiply_by_constant:x0: v_Self -> x1: i32
-    -> Prims.Pure v_Self
-        (f_multiply_by_constant_pre x0 x1)
-        (fun result -> f_multiply_by_constant_post x0 x1 result)
-}
-
-class t_ArrayOperations (v_Self: Type) = {
-  f_ZERO_pre:Prims.unit -> bool;
-  f_ZERO_post:Prims.unit -> v_Self -> bool;
-  f_ZERO:x0: Prims.unit -> Prims.Pure v_Self (f_ZERO_pre x0) (fun result -> f_ZERO_post x0 result);
-  f_to_i32_array_pre:v_Self -> bool;
-  f_to_i32_array_post:v_Self -> t_Array i32 (sz 8) -> bool;
-  f_to_i32_array:x0: v_Self
-    -> Prims.Pure (t_Array i32 (sz 8))
-        (f_to_i32_array_pre x0)
-        (fun result -> f_to_i32_array_post x0 result);
-  f_from_i32_array_pre:t_Array i32 (sz 8) -> bool;
-  f_from_i32_array_post:t_Array i32 (sz 8) -> v_Self -> bool;
-  f_from_i32_array:x0: t_Array i32 (sz 8)
-    -> Prims.Pure v_Self (f_from_i32_array_pre x0) (fun result -> f_from_i32_array_post x0 result)
-}
-
-class t_BitwiseOperations (v_Self: Type) = {
-  f_bitwise_and_with_constant_pre:v_Self -> i32 -> bool;
-  f_bitwise_and_with_constant_post:v_Self -> i32 -> v_Self -> bool;
-  f_bitwise_and_with_constant:x0: v_Self -> x1: i32
-    -> Prims.Pure v_Self
-        (f_bitwise_and_with_constant_pre x0 x1)
-        (fun result -> f_bitwise_and_with_constant_post x0 x1 result);
-  f_shift_right_pre:v_Self -> u8 -> bool;
-  f_shift_right_post:v_Self -> u8 -> v_Self -> bool;
-  f_shift_right:x0: v_Self -> x1: u8
-    -> Prims.Pure v_Self (f_shift_right_pre x0 x1) (fun result -> f_shift_right_post x0 x1 result);
-  f_shift_left_pre:v_Self -> u8 -> bool;
-  f_shift_left_post:v_Self -> u8 -> v_Self -> bool;
-  f_shift_left:x0: v_Self -> x1: u8
-    -> Prims.Pure v_Self (f_shift_left_pre x0 x1) (fun result -> f_shift_left_post x0 x1 result)
-}
-
-class t_CompressionOperations (v_Self: Type) = {
-  f_compress_1_pre:v_Self -> bool;
-  f_compress_1_post:v_Self -> v_Self -> bool;
-  f_compress_1_:x0: v_Self
-    -> Prims.Pure v_Self (f_compress_1_pre x0) (fun result -> f_compress_1_post x0 result);
-  f_compress_pre:u8 -> v_Self -> bool;
-  f_compress_post:u8 -> v_Self -> v_Self -> bool;
-  f_compress:x0: u8 -> x1: v_Self
-    -> Prims.Pure v_Self (f_compress_pre x0 x1) (fun result -> f_compress_post x0 x1 result)
-}
-
 class t_GenericOperations (v_Self: Type) = {
   f_montgomery_multiply_fe_by_fer_pre:v_Self -> i32 -> bool;
   f_montgomery_multiply_fe_by_fer_post:v_Self -> i32 -> v_Self -> bool;
@@ -97,7 +32,52 @@ class t_GenericOperations (v_Self: Type) = {
     -> Prims.Pure v_Self (f_decompress_pre x0 x1) (fun result -> f_decompress_post x0 x1 result)
 }
 
-class t_ModularOperations (v_Self: Type) = {
+class t_Operations (v_Self: Type) = {
+  f_ZERO_pre:Prims.unit -> bool;
+  f_ZERO_post:Prims.unit -> v_Self -> bool;
+  f_ZERO:x0: Prims.unit -> Prims.Pure v_Self (f_ZERO_pre x0) (fun result -> f_ZERO_post x0 result);
+  f_to_i32_array_pre:v_Self -> bool;
+  f_to_i32_array_post:v_Self -> t_Array i32 (sz 8) -> bool;
+  f_to_i32_array:x0: v_Self
+    -> Prims.Pure (t_Array i32 (sz 8))
+        (f_to_i32_array_pre x0)
+        (fun result -> f_to_i32_array_post x0 result);
+  f_from_i32_array_pre:t_Array i32 (sz 8) -> bool;
+  f_from_i32_array_post:t_Array i32 (sz 8) -> v_Self -> bool;
+  f_from_i32_array:x0: t_Array i32 (sz 8)
+    -> Prims.Pure v_Self (f_from_i32_array_pre x0) (fun result -> f_from_i32_array_post x0 result);
+  f_add_constant_pre:v_Self -> i32 -> bool;
+  f_add_constant_post:v_Self -> i32 -> v_Self -> bool;
+  f_add_constant:x0: v_Self -> x1: i32
+    -> Prims.Pure v_Self (f_add_constant_pre x0 x1) (fun result -> f_add_constant_post x0 x1 result);
+  f_add_pre:v_Self -> v_Self -> bool;
+  f_add_post:v_Self -> v_Self -> v_Self -> bool;
+  f_add:x0: v_Self -> x1: v_Self
+    -> Prims.Pure v_Self (f_add_pre x0 x1) (fun result -> f_add_post x0 x1 result);
+  f_sub_pre:v_Self -> v_Self -> bool;
+  f_sub_post:v_Self -> v_Self -> v_Self -> bool;
+  f_sub:x0: v_Self -> x1: v_Self
+    -> Prims.Pure v_Self (f_sub_pre x0 x1) (fun result -> f_sub_post x0 x1 result);
+  f_multiply_by_constant_pre:v_Self -> i32 -> bool;
+  f_multiply_by_constant_post:v_Self -> i32 -> v_Self -> bool;
+  f_multiply_by_constant:x0: v_Self -> x1: i32
+    -> Prims.Pure v_Self
+        (f_multiply_by_constant_pre x0 x1)
+        (fun result -> f_multiply_by_constant_post x0 x1 result);
+  f_bitwise_and_with_constant_pre:v_Self -> i32 -> bool;
+  f_bitwise_and_with_constant_post:v_Self -> i32 -> v_Self -> bool;
+  f_bitwise_and_with_constant:x0: v_Self -> x1: i32
+    -> Prims.Pure v_Self
+        (f_bitwise_and_with_constant_pre x0 x1)
+        (fun result -> f_bitwise_and_with_constant_post x0 x1 result);
+  f_shift_right_pre:v_Self -> u8 -> bool;
+  f_shift_right_post:v_Self -> u8 -> v_Self -> bool;
+  f_shift_right:x0: v_Self -> x1: u8
+    -> Prims.Pure v_Self (f_shift_right_pre x0 x1) (fun result -> f_shift_right_post x0 x1 result);
+  f_shift_left_pre:v_Self -> u8 -> bool;
+  f_shift_left_post:v_Self -> u8 -> v_Self -> bool;
+  f_shift_left:x0: v_Self -> x1: u8
+    -> Prims.Pure v_Self (f_shift_left_pre x0 x1) (fun result -> f_shift_left_post x0 x1 result);
   f_modulo_a_constant_pre:v_Self -> i32 -> bool;
   f_modulo_a_constant_post:v_Self -> i32 -> v_Self -> bool;
   f_modulo_a_constant:x0: v_Self -> x1: i32
@@ -113,10 +93,15 @@ class t_ModularOperations (v_Self: Type) = {
   f_montgomery_reduce:x0: v_Self
     -> Prims.Pure v_Self
         (f_montgomery_reduce_pre x0)
-        (fun result -> f_montgomery_reduce_post x0 result)
-}
-
-class t_NTTOperations (v_Self: Type) = {
+        (fun result -> f_montgomery_reduce_post x0 result);
+  f_compress_1_pre:v_Self -> bool;
+  f_compress_1_post:v_Self -> v_Self -> bool;
+  f_compress_1_:x0: v_Self
+    -> Prims.Pure v_Self (f_compress_1_pre x0) (fun result -> f_compress_1_post x0 result);
+  f_compress_pre:u8 -> v_Self -> bool;
+  f_compress_post:u8 -> v_Self -> v_Self -> bool;
+  f_compress:x0: u8 -> x1: v_Self
+    -> Prims.Pure v_Self (f_compress_pre x0 x1) (fun result -> f_compress_post x0 x1 result);
   f_ntt_layer_1_step_pre:v_Self -> i32 -> i32 -> bool;
   f_ntt_layer_1_step_post:v_Self -> i32 -> i32 -> v_Self -> bool;
   f_ntt_layer_1_step:x0: v_Self -> x1: i32 -> x2: i32
@@ -146,10 +131,7 @@ class t_NTTOperations (v_Self: Type) = {
   f_ntt_multiply:x0: v_Self -> x1: v_Self -> x2: i32 -> x3: i32
     -> Prims.Pure v_Self
         (f_ntt_multiply_pre x0 x1 x2 x3)
-        (fun result -> f_ntt_multiply_post x0 x1 x2 x3 result)
-}
-
-class t_SerializeOperations (v_Self: Type) = {
+        (fun result -> f_ntt_multiply_post x0 x1 x2 x3 result);
   f_serialize_1_pre:v_Self -> bool;
   f_serialize_1_post:v_Self -> u8 -> bool;
   f_serialize_1_:x0: v_Self
@@ -210,21 +192,12 @@ class t_SerializeOperations (v_Self: Type) = {
     -> Prims.Pure v_Self (f_deserialize_12_pre x0) (fun result -> f_deserialize_12_post x0 result)
 }
 
-class t_Operations (v_Self: Type) = {
-  [@@@ FStar.Tactics.Typeclasses.no_method]_super_16550665238208597986:t_ArrayOperations v_Self;
-  [@@@ FStar.Tactics.Typeclasses.no_method]_super_9181983936900423582:t_ArithmeticOperations v_Self;
-  [@@@ FStar.Tactics.Typeclasses.no_method]_super_11057338832248834886:t_ModularOperations v_Self;
-  [@@@ FStar.Tactics.Typeclasses.no_method]_super_5739476159407468282:t_BitwiseOperations v_Self;
-  [@@@ FStar.Tactics.Typeclasses.no_method]_super_13298396156660513588:t_CompressionOperations
-  v_Self;
-  [@@@ FStar.Tactics.Typeclasses.no_method]_super_1988623142765322925:t_NTTOperations v_Self;
-  [@@@ FStar.Tactics.Typeclasses.no_method]_super_18188678553863793517:t_SerializeOperations v_Self;
-  [@@@ FStar.Tactics.Typeclasses.no_method]_super_957087622381469234:Core.Marker.t_Copy v_Self;
-  [@@@ FStar.Tactics.Typeclasses.no_method]_super_2101570567305961368:Core.Clone.t_Clone v_Self
-}
-
 [@@ FStar.Tactics.Typeclasses.tcinstance]
-let impl (#v_T: Type) (#[FStar.Tactics.Typeclasses.tcresolve ()] i1: t_Operations v_T)
+let impl
+      (#v_T: Type)
+      (#[FStar.Tactics.Typeclasses.tcresolve ()] i1: t_Operations v_T)
+      (#[FStar.Tactics.Typeclasses.tcresolve ()] i2: Core.Clone.t_Clone v_T)
+      (#[FStar.Tactics.Typeclasses.tcresolve ()] i3: Core.Marker.t_Copy v_T)
     : t_GenericOperations v_T =
   {
     f_montgomery_multiply_fe_by_fer_pre = (fun (v: v_T) (fer: i32) -> true);
